make ImplVariables a mutable class

disk-betree/ImplCache.i.dfy
@@ -18,16 +18,16 @@ module ImplCache {
 
   method getFreeRef(s: ImplVariables)
   returns (ref : Option<BT.G.Reference>)
-  requires s.Ready?
-  requires IS.WVars(s)
-  ensures ref == ImplModelCache.getFreeRef(IS.IVars(s))
+  requires s.ready
+  requires s.W()
+  ensures ref == ImplModelCache.getFreeRef(s.I())
   {
     ImplModelCache.reveal_getFreeRef();
     var i := 1;
     while true
     invariant i >= 1
-    invariant ImplModelCache.getFreeRefIterate(IS.IVars(s), i)
-           == ImplModelCache.getFreeRef(IS.IVars(s))
+    invariant ImplModelCache.getFreeRefIterate(s.I(), i)
+           == ImplModelCache.getFreeRef(s.I())
     decreases 0x1_0000_0000_0000_0000 - i as int
     {
       var lookup := s.ephemeralIndirectionTable.Get(i);
@@ -43,16 +43,16 @@ module ImplCache {
 
   method getFreeRef2(s: ImplVariables, avoid: BT.G.Reference)
   returns (ref : Option<BT.G.Reference>)
-  requires s.Ready?
-  requires IS.WVars(s)
-  ensures ref == ImplModelCache.getFreeRef2(IS.IVars(s), avoid)
+  requires s.ready
+  requires s.W()
+  ensures ref == ImplModelCache.getFreeRef2(s.I(), avoid)
   {
     ImplModelCache.reveal_getFreeRef2();
     var i := 1;
     while true
     invariant i >= 1
-    invariant ImplModelCache.getFreeRef2Iterate(IS.IVars(s), avoid, i)
-           == ImplModelCache.getFreeRef2(IS.IVars(s), avoid)
+    invariant ImplModelCache.getFreeRef2Iterate(s.I(), avoid, i)
+           == ImplModelCache.getFreeRef2(s.I(), avoid)
     decreases 0x1_0000_0000_0000_0000 - i as int
     {
       var lookup := s.ephemeralIndirectionTable.Get(i);
@@ -67,20 +67,12 @@ module ImplCache {
   }
 
   method write(k: ImplConstants, s: ImplVariables, ref: BT.G.Reference, node: IS.Node)
-  returns (s': ImplVariables)
-  requires s.Ready?
-  requires IS.WVars(s)
-  ensures s'.Ready?
-  ensures s'.ephemeralIndirectionTable == s.ephemeralIndirectionTable
-  // NOALIAS statically enforced no-aliasing would probably help here
-  ensures forall r | r in s.ephemeralIndirectionTable.Repr :: fresh(r) || r in old(s.ephemeralIndirectionTable.Repr)
-  ensures forall r | r in s'.lru.Repr :: fresh(r) || r in old(s.lru.Repr)
-
-  ensures IS.WVars(s')
-  ensures IS.IVars(s') == ImplModelCache.write(Ic(k), old(IS.IVars(s)), ref, node)
-
-  modifies s.ephemeralIndirectionTable.Repr
-  modifies s.lru.Repr
+  requires s.ready
+  requires s.W()
+  modifies s.Repr()
+  ensures s.ready
+  ensures WellUpdated(s)
+  ensures s.I() == ImplModelCache.write(Ic(k), old(s.I()), ref, node)
   {
     ImplModelCache.reveal_write();
 
@@ -90,34 +82,23 @@ module ImplCache {
 
     assume |LruModel.I(s.lru.Queue)| <= 0x10000;
     s.lru.Use(ref);
-    s' := s.(cache := s.cache[ref := node]);
+    s.cache := s.cache[ref := node];
   }
 
   method alloc(k: ImplConstants, s: ImplVariables, node: IS.Node)
-  returns (s': ImplVariables, ref: Option<BT.G.Reference>)
-  requires s.Ready?
-  requires IS.WVars(s)
-
-  ensures s'.Ready?
-  // NOALIAS statically enforced no-aliasing would probably help here
-  ensures s'.ephemeralIndirectionTable.Repr == s.ephemeralIndirectionTable.Repr
-  // NOALIAS statically enforced no-aliasing would probably help here
-  ensures forall r | r in s.ephemeralIndirectionTable.Repr :: fresh(r) || r in old(s.ephemeralIndirectionTable.Repr)
-  ensures forall r | r in s'.lru.Repr :: fresh(r) || r in old(s.lru.Repr)
-
-  ensures IS.WVars(s')
-  ensures (IS.IVars(s'), ref) == ImplModelCache.alloc(Ic(k), old(IS.IVars(s)), node)
-
-  modifies s.ephemeralIndirectionTable.Repr
-  modifies s.lru.Repr
+  returns (ref: Option<BT.G.Reference>)
+  requires s.ready
+  requires s.W()
+  modifies s.Repr()
+  ensures s.ready
+  ensures WellUpdated(s)
+  ensures (s.I(), ref) == ImplModelCache.alloc(Ic(k), old(s.I()), node)
   {
     ImplModelCache.reveal_alloc();
     
     ref := getFreeRef(s);
     if (ref.Some?) {
-      s' := write(k, s, ref.value, node);
-    } else {
-      s' := s;
+      write(k, s, ref.value, node);
     }
   }
 }
