disk-betree/ImplDealloc.i.dfy
@@ -18,18 +18,18 @@ module ImplDealloc {
   import opened NativeTypes
 
   method Deallocable(s: ImplVariables, ref: BT.G.Reference) returns (result: bool)
-  requires WVars(s)
-  requires s.Ready? ==> s.ephemeralIndirectionTable.Inv()
-  ensures result == ImplModelDealloc.deallocable(IVars(s), ref)
+  requires s.W()
+  requires s.ready ==> s.ephemeralIndirectionTable.Inv()
+  ensures result == ImplModelDealloc.deallocable(s.I(), ref)
   {
     if ref == BT.G.Root() {
       return false;
     }
     assert ref != BT.G.Root();
-    if !s.Ready? {
+    if !s.ready {
       return false;
     }
-    assert s.Ready?;
+    assert s.ready;
     var lbaGraph := s.ephemeralIndirectionTable.Get(ref);
     if !lbaGraph.Some? {
       return false;
@@ -42,32 +42,23 @@ module ImplDealloc {
   }
 
   method Dealloc(k: ImplConstants, s: ImplVariables, io: DiskIOHandler, ref: BT.G.Reference)
-  returns (s': ImplVariables)
   requires Inv(k, s)
   requires io.initialized()
-  requires ImplModelDealloc.deallocable(IVars(s), ref)
-  requires io !in VariablesReadSet(s)
+  requires ImplModelDealloc.deallocable(s.I(), ref)
+  requires io !in s.Repr()
   modifies io
-  ensures WVars(s')
-  ensures s'.Ready?
-  ensures (IVars(s'), IIO(io)) == ImplModelDealloc.Dealloc(Ic(k), old(IVars(s)), old(IIO(io)), ref);
-  // NOALIAS statically enforced no-aliasing would probably help here
-  ensures s'.Ready?
-  ensures s'.ephemeralIndirectionTable.Repr == s.ephemeralIndirectionTable.Repr
-  // NOALIAS statically enforced no-aliasing would probably help here
-  ensures forall r | r in s.ephemeralIndirectionTable.Repr :: fresh(r) || r in old(s.ephemeralIndirectionTable.Repr)
-  ensures forall r | r in s'.lru.Repr :: fresh(r) || r in old(s.lru.Repr)
-  modifies s.ephemeralIndirectionTable.Repr
-  modifies s.lru.Repr
+  modifies s.Repr()
+  ensures WellUpdated(s)
+  ensures s.ready
+  ensures (s.I(), IIO(io)) == ImplModelDealloc.Dealloc(Ic(k), old(s.I()), old(IIO(io)), ref);
   {
     ImplModelDealloc.reveal_Dealloc();
 
-    if s.frozenIndirectionTable.Some? {
-      var lbaGraph := s.frozenIndirectionTable.value.Get(ref);
+    if s.frozenIndirectionTable != null {
+      var lbaGraph := s.frozenIndirectionTable.Get(ref);
       if lbaGraph.Some? {
         var (lba, _) := lbaGraph.value;
         if lba.None? {
-          s' := s;
           print "giving up; dealloc can't dealloc because frozen isn't written\n";
           return;
         }
@@ -75,7 +66,6 @@ module ImplDealloc {
     }
 
     if !BC.OutstandingBlockReadsDoesNotHaveRef(s.outstandingBlockReads, ref) {
-      s' := s;
       print "giving up; dealloc can't dealloc because of outstanding read\n";
       return;
     }
@@ -83,17 +73,16 @@ module ImplDealloc {
     var _ := s.ephemeralIndirectionTable.Remove(ref);
 
     s.lru.Remove(ref);
-    s' := s
-      .(cache := MapRemove(s.cache, {ref}));
+    s.cache := MapRemove(s.cache, {ref});
 
-    assume s'.ephemeralIndirectionTable.Contents
-        == MapRemove(old(s'.ephemeralIndirectionTable.Contents), {ref});
+    assume s.ephemeralIndirectionTable.Contents
+        == MapRemove(old(s.ephemeralIndirectionTable.Contents), {ref});
   }
 
   method FindDeallocable(s: ImplVariables) returns (ref: Option<Reference>)
-  requires WFVars(s)
-  requires s.Ready?
-  ensures ref == ImplModelDealloc.FindDeallocable(IVars(s))
+  requires s.WF()
+  requires s.ready
+  ensures ref == ImplModelDealloc.FindDeallocable(s.I())
   {
     ImplModelDealloc.reveal_FindDeallocable();
 
@@ -106,8 +95,8 @@ module ImplDealloc {
     var i: uint64 := 0;
     while i as int < |ephemeralRefs|
     invariant 0 <= i as int <= |ephemeralRefs|
-    invariant ImplModelDealloc.FindDeallocableIterate(IVars(s), ephemeralRefs, i)
-           == ImplModelDealloc.FindDeallocable(IVars(s))
+    invariant ImplModelDealloc.FindDeallocableIterate(s.I(), ephemeralRefs, i)
+           == ImplModelDealloc.FindDeallocable(s.I())
     {
       var ref := ephemeralRefs[i];
       var isDeallocable := Deallocable(s, ref);
