disk-betree/ImplGrow.i.dfy
@@ -20,56 +20,41 @@ module ImplGrow {
 
   /// The root was found to be too big: grow
   method grow(k: ImplConstants, s: ImplVariables)
-  returns (s': ImplVariables)
   requires Inv(k, s)
-  requires s.Ready?
+  requires s.ready
   requires BT.G.Root() in s.cache
-  ensures IS.WVars(s')
-  ensures s'.Ready?
-  ensures IVars(s') == ImplModelGrow.grow(Ic(k), old(IVars(s)))
-  // NOALIAS statically enforced no-aliasing would probably help here
-  ensures forall r | r in s.ephemeralIndirectionTable.Repr :: fresh(r) || r in old(s.ephemeralIndirectionTable.Repr)
-  ensures forall r | r in s'.lru.Repr :: fresh(r) || r in old(s.lru.Repr)
-  modifies s.ephemeralIndirectionTable.Repr
-  modifies s.lru.Repr
+  modifies s.Repr()
+  ensures WellUpdated(s)
+  ensures s.ready
+  ensures s.I() == ImplModelGrow.grow(Ic(k), old(s.I()))
   {
     ImplModelGrow.reveal_grow();
 
-    if s.frozenIndirectionTable.Some? {
-      var rootLbaGraph := s.frozenIndirectionTable.value.Get(BT.G.Root());
+    if s.frozenIndirectionTable != null {
+      var rootLbaGraph := s.frozenIndirectionTable.Get(BT.G.Root());
       if rootLbaGraph.Some? {
         var (lba, _) := rootLbaGraph.value;
         if lba.None? {
-          s' := s;
           print "giving up; grow can't run because frozen isn't written\n";
           return;
         }
       }
     }
 
-    var s0 := flushRootBucket(k, s);
-    ImplModelFlushRootBucket.flushRootBucketCorrect(Ic(k), IVars(s));
+    ImplModelFlushRootBucket.flushRootBucketCorrect(Ic(k), s.I());
+    flushRootBucket(k, s);
 
-    var oldroot := s0.cache[BT.G.Root()];
-    var s1, newref := alloc(k, s0, oldroot);
-
-    // NOALIAS statically enforced no-aliasing would probably help here
-    /* (doc) assert forall r | r in s1.ephemeralIndirectionTable.Repr :: fresh(r) || r in old(s0.ephemeralIndirectionTable.Repr); */
-    /* (doc) assert forall r | r in s1.ephemeralIndirectionTable.Repr :: fresh(r) || r in s0.ephemeralIndirectionTable.Repr; */
+    var oldroot := s.cache[BT.G.Root()];
+    var newref := alloc(k, s, oldroot);
 
     match newref {
       case None => {
-        s' := s1;
         print "giving up; could not allocate ref\n";
       }
       case Some(newref) => {
         var newroot := IM.Node([], Some([newref]), [KMTable.Empty()]);
 
-        // NOALIAS statically enforced no-aliasing would probably help here
-        /* (doc) assert forall r | r in s1.ephemeralIndirectionTable.Repr :: fresh(r) || r in old(s0.ephemeralIndirectionTable.Repr); */
-        /* (doc) assert forall r | r in s1.ephemeralIndirectionTable.Repr :: fresh(r) || r in s0.ephemeralIndirectionTable.Repr; */
-
-        s' := write(k, s1, BT.G.Root(), newroot);
+        write(k, s, BT.G.Root(), newroot);
       }
     }
   }
