disk-betree/ImplQuery.i.dfy
@@ -33,8 +33,8 @@ module ImplQuery {
   method TryRootBucketLookup(k: ImplConstants, s: ImplVariables, key: MS.Key)
   returns (res: Option<MS.Value>)
   requires Inv(k, s)
-  requires s.Ready?
-  ensures res == ImplModelQuery.TryRootBucketLookup(Ic(k), IVars(s), key)
+  requires s.ready
+  ensures res == ImplModelQuery.TryRootBucketLookup(Ic(k), s.I(), key)
   {
     var qres := TTT.Query(s.rootBucket, key);
     if (qres.ValueForKey?) {
@@ -45,25 +45,24 @@ module ImplQuery {
   }
 
   method query(k: ImplConstants, s: ImplVariables, io: DiskIOHandler, key: MS.Key)
-  returns (s': ImplVariables, res: Option<MS.Value>)
+  returns (res: Option<MS.Value>)
   requires io.initialized()
   requires Inv(k, s)
-  requires io !in VariablesReadSet(s)
+  requires io !in s.Repr()
   modifies io
-  modifies if s.Ready? then s.lru.Repr else {}
-  ensures WVars(s')
-  ensures (IVars(s'), res, IIO(io)) == ImplModelQuery.query(Ic(k), old(IVars(s)), old(IIO(io)), key)
+  modifies s.Repr()
+  ensures WellUpdated(s)
+  ensures (s.I(), res, IIO(io)) == ImplModelQuery.query(Ic(k), old(s.I()), old(IIO(io)), key)
   {
     ImplModelQuery.reveal_query();
     ImplModelQuery.reveal_queryIterate();
 
-    if (s.Unready?) {
-      s' := PageInIndirectionTableReq(k, s, io);
+    if (!s.ready) {
+      PageInIndirectionTableReq(k, s, io);
       res := None;
     } else {
       var rootLookup := TryRootBucketLookup(k, s, key);
       if (rootLookup.Some?) {
-        s' := s;
         res := rootLookup;
         return;
       }
@@ -74,39 +73,37 @@ module ImplQuery {
 
       while true
       invariant Inv(k, s)
-      invariant s.Ready?
+      invariant s.ready
       invariant ref in IM.IIndirectionTable(IIndirectionTable(s.ephemeralIndirectionTable)).graph
       invariant io.initialized()
-      invariant ImplModelQuery.query(Ic(k), old(IVars(s)), old(IIO(io)), key)
-             == ImplModelQuery.queryIterate(Ic(k), IVars(s), key, msg, ref, IIO(io), counter)
+      invariant ImplModelQuery.query(Ic(k), old(s.I()), old(IIO(io)), key)
+             == ImplModelQuery.queryIterate(Ic(k), s.I(), key, msg, ref, IIO(io), counter)
       invariant counter as int >= 0
-      invariant io !in VariablesReadSet(s)
-      invariant forall r | r in s.lru.Repr :: r in old(s.lru.Repr) || fresh(r)
+      invariant io !in s.Repr()
+      invariant WellUpdated(s)
       decreases counter as int
       {
         if counter == 0 {
-          s' := s;
           res := None;
           return;
         }
 
         if (ref !in s.cache) {
           if |s.cache| + |s.outstandingBlockReads| <= MaxCacheSize() - 1 {
-            s' := PageInReq(k, s, io, ref);
+            PageInReq(k, s, io, ref);
             res := None;
             return;
           } else {
-            s' := s;
             res := None;
             return;
           }
         } else {
           var node := s.cache[ref];
 
-          ghost var oldIVars := IVars(s);
+          ghost var oldIVars := s.I();
           LruModel.LruUse(s.lru.Queue, ref);
           s.lru.Use(ref);
-          assert IM.IVars(oldIVars) == IM.IVars(IVars(s));
+          assert IM.IVars(oldIVars) == IM.IVars(s.I());
 
           var r := Pivots.ComputeRoute(node.pivotTable, key);
           var bucket := node.buckets[r];
@@ -115,16 +112,14 @@ module ImplQuery {
           var newmsg := if kmtMsg.Some? then Messages.Merge(msg, kmtMsg.value) else msg;
 
           if (newmsg.Define?) {
-            s' := s;
             res := Some(newmsg.value);
             return;
           } else {
             if node.children.Some? {
-              ImplModelCache.lemmaChildInGraph(Ic(k), IVars(s), ref, node.children.value[r]);
+              ImplModelCache.lemmaChildInGraph(Ic(k), s.I(), ref, node.children.value[r]);
               counter := counter - 1;
               ref := node.children.value[r];
             } else {
-              s' := s;
               res := Some(MS.V.DefaultValue());
               return;
             }
